Esempio:\newline
\begin{thm}$\displaystyle \sum_{i = 0} ^ n i = \frac{n(n + 1)}{2}$ \end{thm}

\begin{proof}
Per $n = 0 \quad \displaystyle \sum_{i = 0} ^ 0 i = \frac{0(0 + 1)}{2} \quad 0 = 0$ vero

Se $\displaystyle \sum_{i = 0} ^ n i = \frac{n(n+1)}{2}$ allora
$\displaystyle \sum_{i = 0} ^ {n+1} i = \frac{(n+1)(n+2)}{2}$
\begin{equation*}
\begin{split}
  \sum_{i = 0}^{n+1} i & = \sum_{i = 0} ^ n + (n+1) \\
                     & = \frac{n(n+1)}{2} + (n+1) \\
                     & = \frac{n(n+1) + 2(n+1)}{2} \\
                     & = \frac{(n+1)(n+2)}{2} \\
\end{split}
\end{equation*}
\end{proof}
