%Dimostrazione per induzione esempio5
\begin{thm}
    $\sum _ {k=0} ^ n (3k+1) = \frac{3n^2+5n+2}{2}$
\end{thm}

\begin{proof}
Caso base $n = 0$:
\begin{equation*}
    \sum _ {k = 0} ^ 0 (3k+1) = \frac{0+0+2}{2} \quad 1 = 1 \text{vero}
\end{equation*}
Caso passo:
\quad Ipotesi:$\sum _ {k=0} ^ n (3k+1) = \frac{3n^2+5n+2}{2}$ \newline
\quad Tesi:$\sum _ {k=0} ^ {n+1} (3k+1) = \frac{3(n+1)^2+5n+5+2}{2} = \frac{3n^2+11n+10}{2}$
\begin{equation*}
\begin{split}
\sum _ {k=0} ^ {n+1} (3k+1) & = \sum _ {k = 0} ^ n (3k+1) + 3(n+1)+1\\
                            & = \frac{3n^2+5n+2}{2} + 3n+4\\
                            & = \frac{3n^2+5n+2+6n+8}{2}\\
                            & = \frac{3n^2+11+10}{2}\\
\end{split}
\end{equation*}
\end{proof}
